src/lowparse/pulse/LowParse.PulseParse.BitSum.fst
@@ -1,0 +1,49 @@
+module LowParse.PulseParse.BitSum
+#lang-pulse
+include LowParse.Spec.BitSum
+open FStar.Tactics.V2
+open Pulse.Lib.Pervasives open Pulse.Lib.Slice.Util open Pulse.Lib.Trade
+open Pulse.Lib.Slice
+open LowParse.Spec.Base
+
+module SZ = FStar.SizeT
+module Trade = Pulse.Lib.Trade.Util
+module S = Pulse.Lib.Slice
+module LPS = LowParse.Pulse.Base
+module LPC = LowParse.Pulse.Combinators
+module PPB = LowParse.PulseParse.Base
+module PPC = LowParse.PulseParse.Combinators
+
+module LPB = LowParse.Pulse.BitSum
+
+inline_for_extraction
+let read_synth_cont_ifthenelse
+  (#t: Type0)
+  (x: Ghost.erased t)
+: Tot (if_combinator_weak (PPC.read_synth_cont_t #t x))
+= fun cond iftrue iffalse t' g' -> if cond then iftrue () t' g' else iffalse () t' g'
+
+inline_for_extraction
+let read_bitsum'
+  (#t: eqtype)
+  (#tot: pos)
+  (#cl: uint_t tot t)
+  (#b: bitsum' cl tot)
+  (d: destr_bitsum'_t b)
+  (#k: Ghost.erased parser_kind)
+  (#p: parser k t)
+  (r: PPB.reader p)
+: Tot (PPB.reader (parse_bitsum' b p))
+= PPC.read_synth
+    (PPC.read_filter
+      r
+      (filter_bitsum' b)
+    )
+    (synth_bitsum'_injective b; synth_bitsum' b)
+    (synth_bitsum'_recip_inverse b; synth_bitsum'_recip b)
+    (
+      d
+        (PPC.read_synth_cont_t #(bitsum'_type b))
+        (read_synth_cont_ifthenelse #(bitsum'_type b))
+        (PPC.read_synth_cont_init)
+    )
