src/lowparse/pulse/LowParse.PulseParse.Combinators.fst
@@ -1,0 +1,430 @@
+module LowParse.PulseParse.Combinators
+#lang-pulse
+include LowParse.Spec.Combinators
+open FStar.Tactics.V2
+open Pulse.Lib.Pervasives open Pulse.Lib.Slice.Util open Pulse.Lib.Trade
+open Pulse.Lib.Slice
+open LowParse.Spec.Base
+
+module SZ = FStar.SizeT
+module Trade = Pulse.Lib.Trade.Util
+module S = Pulse.Lib.Slice
+module LPS = LowParse.Pulse.Base
+module LPC = LowParse.Pulse.Combinators
+module PPB = LowParse.PulseParse.Base
+
+(* ret / empty *)
+
+inline_for_extraction
+fn leaf_read_ret
+  (#t: Type0)
+  (x: t)
+  (v_unique: (v' : t) -> Lemma (x == v'))
+: PPB.leaf_reader #t #parse_ret_kind (parse_ret x)
+= (input: slice byte)
+  (#pm: _)
+  (#v: _)
+{
+  v_unique v;
+  x
+}
+
+inline_for_extraction
+let read_ret
+  (#t: Type0)
+  (x: t)
+  (v_unique: (v' : t) -> Lemma (x == v'))
+: Tot (PPB.reader (parse_ret x))
+= PPB.reader_of_leaf_reader (leaf_read_ret x v_unique)
+
+inline_for_extraction
+let leaf_read_empty : PPB.leaf_reader parse_empty = leaf_read_ret () (fun _ -> ())
+
+inline_for_extraction
+let read_empty : PPB.reader parse_empty = PPB.reader_of_leaf_reader leaf_read_empty
+
+(* pts_to_parsed synth combinators *)
+
+ghost
+fn pts_to_parsed_synth_intro
+  (#t #t': Type0)
+  (#k: parser_kind)
+  (p: parser k t)
+  (f: (t -> GTot t') { k.parser_kind_injective ==> synth_injective f })
+  (f': (t' -> GTot t) { synth_inverse f f' })
+  (input: slice byte)
+  (#pm: perm)
+  (#v: t)
+  requires PPB.pts_to_parsed p input #pm v
+  ensures PPB.pts_to_parsed (parse_synth p f) input #pm (f v)
+{
+  unfold (PPB.pts_to_parsed p input #pm v);
+  with w . assert (pts_to input #pm w);
+  parse_synth_eq p f w;
+  fold (PPB.pts_to_parsed (parse_synth p f) input #pm (f v))
+}
+
+ghost
+fn pts_to_parsed_synth_elim
+  (#t #t': Type0)
+  (#k: parser_kind)
+  (p: parser k t)
+  (f: (t -> GTot t') { synth_injective f })
+  (f': (t' -> GTot t) { synth_inverse f f' })
+  (input: slice byte)
+  (#pm: perm)
+  (v: t)
+  requires PPB.pts_to_parsed (parse_synth p f) input #pm (f v)
+  ensures PPB.pts_to_parsed p input #pm v
+{
+  unfold (PPB.pts_to_parsed (parse_synth p f) input #pm (f v));
+  with w . assert (pts_to input #pm w);
+  parse_synth_eq p f w;
+  fold (PPB.pts_to_parsed p input #pm v)
+}
+
+ghost
+fn pts_to_parsed_synth_trade
+  (#t #t': Type0)
+  (#k: parser_kind)
+  (p: parser k t)
+  (f: (t -> GTot t') { synth_injective f })
+  (f': (t' -> GTot t) { synth_inverse f f' })
+  (input: slice byte)
+  (#pm: perm)
+  (#v: t)
+  requires PPB.pts_to_parsed p input #pm v
+  ensures PPB.pts_to_parsed (parse_synth p f) input #pm (f v) **
+    trade (PPB.pts_to_parsed (parse_synth p f) input #pm (f v))
+          (PPB.pts_to_parsed p input #pm v)
+{
+  pts_to_parsed_synth_intro p f f' input;
+  intro
+    (Trade.trade
+      (PPB.pts_to_parsed (parse_synth p f) input #pm (f v))
+      (PPB.pts_to_parsed p input #pm v)
+    )
+    #emp
+    fn _ {
+      pts_to_parsed_synth_elim p f f' input v
+    };
+}
+
+ghost
+fn pts_to_parsed_synth_l2r
+  (#t #t': Type0)
+  (#k: parser_kind)
+  (p: parser k t)
+  (f: (t -> GTot t') { synth_injective f })
+  (f': (t' -> GTot t) { synth_inverse f f' })
+  (input: slice byte)
+  (#pm: perm)
+  (#v: t')
+  requires PPB.pts_to_parsed (parse_synth p f) input #pm v
+  ensures PPB.pts_to_parsed p input #pm (f' v)
+{
+  unfold (PPB.pts_to_parsed (parse_synth p f) input #pm v);
+  with w . assert (pts_to input #pm w);
+  parse_synth_eq p f w;
+  let v1 = Ghost.hide (fst (Some?.v (parse p w)));
+  assert pure (f v1 == v);
+  assert pure (f (f' v) == v);
+  fold (PPB.pts_to_parsed p input #pm (f' v))
+}
+
+ghost
+fn pts_to_parsed_synth_r2l
+  (#t #t': Type0)
+  (#k: parser_kind)
+  (p: parser k t)
+  (f: (t -> GTot t') { synth_injective f })
+  (f': (t' -> GTot t) { synth_inverse f f' })
+  (input: slice byte)
+  (#pm: perm)
+  (v: t')
+  requires PPB.pts_to_parsed p input #pm (f' v)
+  ensures PPB.pts_to_parsed (parse_synth p f) input #pm v
+{
+  unfold (PPB.pts_to_parsed p input #pm (f' v));
+  with w . assert (pts_to input #pm w);
+  parse_synth_eq p f w;
+  fold (PPB.pts_to_parsed (parse_synth p f) input #pm v)
+}
+
+ghost
+fn pts_to_parsed_synth_l2r_trade
+  (#t #t': Type0)
+  (#k: parser_kind)
+  (p: parser k t)
+  (f: (t -> GTot t') { synth_injective f })
+  (f': (t' -> GTot t) { synth_inverse f f' })
+  (input: slice byte)
+  (#pm: perm)
+  (#v: t')
+  requires PPB.pts_to_parsed (parse_synth p f) input #pm v
+  ensures PPB.pts_to_parsed p input #pm (f' v) **
+    trade (PPB.pts_to_parsed p input #pm (f' v))
+          (PPB.pts_to_parsed (parse_synth p f) input #pm v)
+{
+  pts_to_parsed_synth_l2r p f f' input;
+  intro
+    (Trade.trade
+      (PPB.pts_to_parsed p input #pm (f' v))
+      (PPB.pts_to_parsed (parse_synth p f) input #pm v)
+    )
+    #emp
+    fn _ {
+      pts_to_parsed_synth_r2l p f f' input v
+    };
+}
+
+(* pts_to_parsed filter combinators *)
+
+ghost
+fn pts_to_parsed_filter_intro
+  (#t: Type0)
+  (#k: parser_kind)
+  (p: parser k t)
+  (f: (t -> GTot bool))
+  (input: slice byte)
+  (#pm: perm)
+  (#v: t)
+  requires PPB.pts_to_parsed p input #pm v ** pure (f v == true)
+  ensures exists* (v': parse_filter_refine f) .
+    PPB.pts_to_parsed (parse_filter p f) input #pm v' ** pure ((v' <: t) == v)
+{
+  unfold (PPB.pts_to_parsed p input #pm v);
+  with w . assert (pts_to input #pm w);
+  parse_filter_eq p f w;
+  fold (PPB.pts_to_parsed (parse_filter p f) input #pm (v <: parse_filter_refine f))
+}
+
+ghost
+fn pts_to_parsed_filter_elim
+  (#t: Type0)
+  (#k: parser_kind)
+  (p: parser k t)
+  (f: (t -> GTot bool))
+  (input: slice byte)
+  (#pm: perm)
+  (#v: parse_filter_refine f)
+  requires PPB.pts_to_parsed (parse_filter p f) input #pm v
+  ensures PPB.pts_to_parsed p input #pm v
+{
+  unfold (PPB.pts_to_parsed (parse_filter p f) input #pm v);
+  with w . assert (pts_to input #pm w);
+  parse_filter_eq p f w;
+  fold (PPB.pts_to_parsed p input #pm (v <: t))
+}
+
+ghost
+fn pts_to_parsed_filter_elim_trade
+  (#t: Type0)
+  (#k: parser_kind)
+  (p: parser k t)
+  (f: (t -> GTot bool))
+  (input: slice byte)
+  (#pm: perm)
+  (#v: parse_filter_refine f)
+  requires PPB.pts_to_parsed (parse_filter p f) input #pm v
+  ensures exists* (v': t) .
+    PPB.pts_to_parsed p input #pm v' **
+    Trade.trade (PPB.pts_to_parsed p input #pm v')
+                (PPB.pts_to_parsed (parse_filter p f) input #pm v) **
+    pure (v' == (v <: t))
+{
+  pts_to_parsed_filter_elim p f input;
+  intro
+    (Trade.trade
+      (PPB.pts_to_parsed p input #pm (v <: t))
+      (PPB.pts_to_parsed (parse_filter p f) input #pm v)
+    )
+    #emp
+    fn _ {
+      pts_to_parsed_filter_intro p f input
+    };
+}
+
+(* read combinators *)
+
+inline_for_extraction
+let read_synth_cont_t
+  (#t: Type0)
+  (x: t)
+= (t': Type0) -> (g': ((y: t { y == x }) -> t')) -> (y': t' { y' == g' x })
+
+inline_for_extraction
+let read_synth_cont
+  (#t1 #t2: Type0)
+  (f2: (t1 -> GTot t2))
+  (f2': ((x: t1) -> read_synth_cont_t (f2 x)))
+  (x1: Ghost.erased t1)
+  (t': Type0)
+  (g: ((x2: t2 { x2 == f2 x1 }) -> Tot t'))
+  (x1': t1 { x1' == Ghost.reveal x1 })
+: Tot t'
+= f2' x1' t' g
+
+inline_for_extraction
+fn read_synth
+  (#k1: Ghost.erased parser_kind) (#t1: Type0) (#p1: parser k1 t1) (r: PPB.reader p1)
+  (#t2: Type0) (f2: (t1 -> GTot t2) { synth_injective f2 })
+  (f1: (t2 -> GTot t1) { synth_inverse f2 f1 })
+  (f2': ((x: t1) -> read_synth_cont_t (f2 x)))
+: PPB.reader #t2 #k1 (parse_synth p1 f2)
+= (input: slice byte)
+  (#pm: _)
+  (#v: _)
+  (t': Type0)
+  (g: _)
+{
+  pts_to_parsed_synth_l2r_trade p1 f2 f1 input;
+  let res = r input #pm #(f1 v) t' (read_synth_cont f2 f2' (f1 v) t' g);
+  Trade.elim _ _;
+  res
+}
+
+inline_for_extraction
+let read_synth_cont_init
+  (#t: Type0)
+  (x: t)
+: Tot (read_synth_cont_t #t x)
+= fun t' g' -> g' x
+
+inline_for_extraction
+let read_synth'
+  (#k1: Ghost.erased parser_kind) (#t1: Type0) (#p1: parser k1 t1) (r: PPB.reader p1)
+  (#t2: Type0) (f2: (t1 -> Tot t2) { synth_injective f2 })
+  (f1: (t2 -> GTot t1) { synth_inverse f2 f1 })
+: PPB.reader #t2 #k1 (parse_synth p1 f2)
+= read_synth r f2 f1 (fun x -> read_synth_cont_init (f2 x))
+
+inline_for_extraction
+let read_filter_cont
+  (#t: Type0)
+  (f: t -> GTot bool)
+  (v: Ghost.erased (parse_filter_refine f))
+  (t': Type0)
+  (g: (x: parse_filter_refine f { x == Ghost.reveal v }) -> t')
+  (x: t { x == Ghost.reveal #t (Ghost.hide #t (Ghost.reveal v)) })
+: Tot t'
+= g x
+
+inline_for_extraction
+fn read_filter
+  (#k1: Ghost.erased parser_kind) (#t1: Type0) (#p1: parser k1 t1) (r: PPB.reader p1)
+  (f: (t1 -> GTot bool))
+: PPB.reader #(parse_filter_refine f) #(parse_filter_kind k1) (parse_filter p1 f)
+= (input: slice byte)
+  (#pm: _)
+  (#v: _)
+  (t': Type0)
+  (g: _)
+{
+  pts_to_parsed_filter_elim p1 f input;
+  let res = r input #pm #(Ghost.hide (Ghost.reveal v)) t' (read_filter_cont f v t' g);
+  pts_to_parsed_filter_intro p1 f input;
+  res
+}
+
+(* validate combinators *)
+
+inline_for_extraction
+fn validate_filter
+  (#t: Type0)
+  (#k: Ghost.erased parser_kind)
+  (#p: parser k t)
+  (w: LPS.validator p)
+  (r: PPB.leaf_reader p)
+  (f: (t -> GTot bool))
+  (f': (x: t) -> (y: bool { y == f x }))
+  (_: squash (k.parser_kind_subkind == Some ParserStrong))
+: LPS.validator #_ #(parse_filter_kind k) (parse_filter p f)
+=
+  (input: slice byte)
+  (poffset: _)
+  (#offset: _)
+  (#pm: perm)
+  (#v: Ghost.erased bytes)
+{
+  parse_filter_eq p f (Seq.slice v (SZ.v offset) (Seq.length v));
+  let offset = !poffset;
+  let is_valid = w input poffset;
+  if is_valid {
+    let off = !poffset;
+    let x = PPB.read_parsed_from_validator_success r input offset off;
+    f' x
+  } else {
+    false
+  }
+}
+
+inline_for_extraction
+let validate_filter'
+  (#t: Type0)
+  (#k: Ghost.erased parser_kind)
+  (#p: parser k t)
+  (w: LPS.validator p)
+  (r: PPB.leaf_reader p)
+  (f: (t -> bool))
+  (sq: squash (k.parser_kind_subkind == Some ParserStrong))
+: LPS.validator #_ #(parse_filter_kind k) (parse_filter p f)
+= validate_filter w r f (fun x -> f x) sq
+
+inline_for_extraction
+fn validate_dtuple2
+  (#t1: Type0)
+  (#t2: t1 -> Type0)
+  (#k1: Ghost.erased parser_kind)
+  (#p1: parser k1 t1)
+  (v1: LPS.validator p1)
+  (r1: PPB.leaf_reader p1)
+  (#k2: Ghost.erased parser_kind)
+  (#p2: ((x: t1) -> parser k2 (t2 x)))
+  (v2: ((x: t1) -> LPS.validator (p2 x)))
+  (_: squash (k1.parser_kind_subkind == Some ParserStrong))
+: LPS.validator #(dtuple2 t1 t2) #(and_then_kind k1 k2) (parse_dtuple2 #k1 #t1 p1 #k2 #t2 p2)
+=
+  (input: slice byte)
+  (poffset: _)
+  (#offset: _)
+  (#pm: perm)
+  (#v: Ghost.erased bytes)
+{
+  parse_dtuple2_eq p1 p2 (Seq.slice v (SZ.v offset) (Seq.length v));
+  let offset = !poffset;
+  let is_valid1 = v1 input poffset;
+  if is_valid1 {
+    let off = !poffset;
+    let x = PPB.read_parsed_from_validator_success r1 input offset off;
+    v2 x input poffset
+  } else {
+    false
+  }
+}
+
+inline_for_extraction
+fn jump_dtuple2
+  (#t1: Type0)
+  (#t2: t1 -> Type0)
+  (#k1: Ghost.erased parser_kind)
+  (#p1: parser k1 t1)
+  (v1: LPS.jumper p1)
+  (r1: PPB.leaf_reader p1)
+  (#k2: Ghost.erased parser_kind)
+  (#p2: (x: t1) -> parser k2 (t2 x))
+  (v2: (x: t1) -> LPS.jumper (p2 x))
+  (_: squash (k1.parser_kind_subkind == Some ParserStrong))
+: LPS.jumper #(dtuple2 t1 t2) #(and_then_kind k1 k2) (parse_dtuple2 #k1 #t1 p1 #k2 #t2 p2)
+=
+  (input: slice byte)
+  (offset: SZ.t)
+  (#pm: perm)
+  (#v: Ghost.erased bytes)
+{
+  parse_dtuple2_eq p1 p2 (Seq.slice v (SZ.v offset) (Seq.length v));
+  pts_to_len input;
+  let off1 = v1 input offset;
+  let x = PPB.read_parsed_from_validator_success r1 input offset off1;
+  v2 x input off1
+}
