src/lowparse/pulse/LowParse.PulseParse.VCList.fst
@@ -1,0 +1,270 @@
+module LowParse.PulseParse.VCList
+#lang-pulse
+include LowParse.Spec.VCList
+open FStar.Tactics.V2
+open Pulse.Lib.Pervasives
+open Pulse.Lib.Slice.Util
+open Pulse.Lib.Trade
+open Pulse.Lib.Slice
+open LowParse.Spec.Base
+open LowParse.Spec.Combinators
+
+module SZ = FStar.SizeT
+module R = Pulse.Lib.Reference
+module Trade = Pulse.Lib.Trade.Util
+module S = Pulse.Lib.Slice
+module LPS = LowParse.Pulse.Base
+module PPB = LowParse.PulseParse.Base
+module PPC = LowParse.PulseParse.Combinators
+module LPV = LowParse.Pulse.VCList
+
+(* pts_to_parsed for nlist 1: convert between pts_to_parsed p and pts_to_parsed (parse_nlist 1 p) *)
+
+ghost
+fn pts_to_parsed_nlist_1_intro
+  (#t: Type0)
+  (#k: parser_kind)
+  (p: parser k t)
+  (input: slice byte)
+  (#pm: perm)
+  (#v: t)
+  requires PPB.pts_to_parsed p input #pm v
+  ensures exists* v' .
+    PPB.pts_to_parsed (parse_nlist 1 p) input #pm v' **
+    trade (PPB.pts_to_parsed (parse_nlist 1 p) input #pm v')
+      (PPB.pts_to_parsed p input #pm v) **
+    pure ((v' <: list t) == [v])
+{
+  unfold (PPB.pts_to_parsed p input #pm v);
+  with w . assert (pts_to input #pm w);
+  parse_nlist_eq 1 p w;
+  parse_synth_eq p LPV.synth_nlist_1 w;
+  let v' : Ghost.erased (nlist 1 t) = Ghost.hide [v];
+  fold (PPB.pts_to_parsed (parse_nlist 1 p) input #pm v');
+  intro
+    (Trade.trade
+      (PPB.pts_to_parsed (parse_nlist 1 p) input #pm v')
+      (PPB.pts_to_parsed p input #pm v)
+    )
+    #emp
+    fn _ {
+      unfold (PPB.pts_to_parsed (parse_nlist 1 p) input #pm v');
+      with w' . assert (pts_to input #pm w');
+      parse_nlist_eq 1 p w';
+      parse_synth_eq p LPV.synth_nlist_1 w';
+      fold (PPB.pts_to_parsed p input #pm v)
+    };
+}
+
+ghost
+fn pts_to_parsed_nlist_1_elim
+  (#t: Type0)
+  (#k: parser_kind)
+  (p: parser k t)
+  (input: slice byte)
+  (#pm: perm)
+  (#v: nlist 1 t)
+  requires PPB.pts_to_parsed (parse_nlist 1 p) input #pm v
+  ensures exists* v' .
+    PPB.pts_to_parsed p input #pm v' **
+    trade (PPB.pts_to_parsed p input #pm v')
+      (PPB.pts_to_parsed (parse_nlist 1 p) input #pm v) **
+    pure (v == [v'])
+{
+  unfold (PPB.pts_to_parsed (parse_nlist 1 p) input #pm v);
+  with w . assert (pts_to input #pm w);
+  parse_nlist_eq 1 p w;
+  parse_synth_eq p LPV.synth_nlist_1 w;
+  let v' = Ghost.hide (List.Tot.hd v);
+  fold (PPB.pts_to_parsed p input #pm v');
+  intro
+    (Trade.trade
+      (PPB.pts_to_parsed p input #pm v')
+      (PPB.pts_to_parsed (parse_nlist 1 p) input #pm v)
+    )
+    #emp
+    fn _ {
+      unfold (PPB.pts_to_parsed p input #pm v');
+      with w' . assert (pts_to input #pm w');
+      parse_nlist_eq 1 p w';
+      parse_synth_eq p LPV.synth_nlist_1 w';
+      fold (PPB.pts_to_parsed (parse_nlist 1 p) input #pm v)
+    };
+}
+
+(* pts_to_parsed ext for nlist: convert between equivalent nlist parsers *)
+
+let pts_to_parsed_nlist_ext_aux
+  (#t: Type0)
+  (#k1: parser_kind) (#p1: parser k1 t)
+  (#k2: parser_kind) (#p2: parser k2 t)
+  (n: nat)
+  (prf: (b: bytes) -> Lemma (parse p1 b == parse p2 b))
+  (b: bytes)
+: Lemma (parse (parse_nlist n p1) b == parse (parse_nlist n p2) b)
+= parse_nlist_ext n p1 p2 b (fun b' -> prf b')
+
+ghost
+fn pts_to_parsed_nlist_ext
+  (#t: Type0)
+  (#k1: parser_kind) (#p1: parser k1 t)
+  (#k2: parser_kind) (#p2: parser k2 t)
+  (n: nat)
+  (prf: (b: bytes) -> Lemma (parse p1 b == parse p2 b))
+  (input: slice byte)
+  (#pm: perm)
+  (#v: nlist n t)
+  requires PPB.pts_to_parsed (parse_nlist n p1) input #pm v
+  ensures PPB.pts_to_parsed (parse_nlist n p2) input #pm v
+{
+  Classical.forall_intro (pts_to_parsed_nlist_ext_aux #t #k1 #p1 #k2 #p2 n prf);
+  PPB.pts_to_parsed_ext (parse_nlist n p2) input
+}
+
+(* nlist_hd_tl for pts_to_parsed: split a parsed nlist into head and tail sub-slices.
+   Requires ParserStrong to split raw bytes at the correct boundary. *)
+
+let nlist_hd_tl_post'
+  (#t: Type0)
+  (#k: parser_kind)
+  (p: parser k t)
+  (sq: squash (k.parser_kind_subkind == Some ParserStrong))
+  (n: pos)
+  (input: slice byte)
+  (pm: perm)
+  (v: (nlist n t))
+  (hd tl: slice byte)
+: slprop
+= PPB.pts_to_parsed p hd #(pm /. 2.0R) (List.Tot.hd v) **
+  PPB.pts_to_parsed (parse_nlist (n - 1) p) tl #(pm /. 2.0R) (List.Tot.tl v) **
+  Trade.trade
+    (PPB.pts_to_parsed p hd #(pm /. 2.0R) (List.Tot.hd v) **
+      PPB.pts_to_parsed (parse_nlist (n - 1) p) tl #(pm /. 2.0R) (List.Tot.tl v))
+    (PPB.pts_to_parsed (parse_nlist n p) input #pm v)
+
+let nlist_hd_tl_post
+  (#t: Type0)
+  (#k: parser_kind)
+  (p: parser k t)
+  (sq: squash (k.parser_kind_subkind == Some ParserStrong))
+  (n: pos)
+  (input: slice byte)
+  (pm: perm)
+  (v: (nlist n t))
+  (hd_tl: (slice byte & slice byte))
+: slprop
+= nlist_hd_tl_post' p sq n input pm v (fst hd_tl) (snd hd_tl)
+
+inline_for_extraction
+fn nlist_hd_tl
+  (#t: Type0)
+  (#k: Ghost.erased parser_kind)
+  (#p: parser k t)
+  (sq: squash (k.parser_kind_subkind == Some ParserStrong))
+  (j: LPS.jumper p)
+  (n: Ghost.erased pos)
+  (input: slice byte)
+  (#pm: perm)
+  (#v: Ghost.erased (nlist n t))
+requires
+  PPB.pts_to_parsed (parse_nlist n p) input #pm v
+returns res : (slice byte & slice byte)
+ensures
+  nlist_hd_tl_post p sq n input pm v res
+{
+  PPB.pts_to_parsed_elim input;
+  with w . assert (pts_to input #pm w);
+  parse_nlist_eq (Ghost.reveal n) p w;
+  parser_kind_prop_equiv k p;
+  let off = j input 0sz;
+  let input1, input2 = split_trade input off;
+  with w1 . assert (pts_to input1 #pm w1);
+  with w2 . assert (pts_to input2 #pm w2);
+  parse_strong_prefix p w w1;
+  let vh = Ghost.hide (List.Tot.hd (Ghost.reveal v));
+  let vt : Ghost.erased (nlist (n - 1) t) = Ghost.hide (List.Tot.tl (Ghost.reveal v));
+  PPB.pts_to_parsed_intro p input1 vh;
+  PPB.pts_to_parsed_intro (parse_nlist (n - 1) p) input2 vt;
+  // Trade chain: (parsed hd ** parsed tl) -> (pts_to input1 ** pts_to input2) -> (pts_to input) -> (parsed nlist)
+  Trade.prod
+    (PPB.pts_to_parsed p input1 #(pm /. 2.0R) vh)
+    (pts_to input1 #pm w1)
+    (PPB.pts_to_parsed (parse_nlist (n - 1) p) input2 #(pm /. 2.0R) vt)
+    (pts_to input2 #pm w2);
+  Trade.trans
+    (PPB.pts_to_parsed p input1 #(pm /. 2.0R) vh ** PPB.pts_to_parsed (parse_nlist (n - 1) p) input2 #(pm /. 2.0R) vt)
+    (pts_to input1 #pm w1 ** pts_to input2 #pm w2)
+    (pts_to input #pm w);
+  // Use existing trade from pts_to_parsed_elim: (pts_to input #pm w) -> (parsed nlist)
+  Trade.trans
+    (PPB.pts_to_parsed p input1 #(pm /. 2.0R) vh ** PPB.pts_to_parsed (parse_nlist (n - 1) p) input2 #(pm /. 2.0R) vt)
+    (pts_to input #pm w)
+    (PPB.pts_to_parsed (parse_nlist n p) input #pm v);
+  rewrite each vh as (List.Tot.hd (Ghost.reveal v));
+  rewrite each vt as (List.Tot.tl (Ghost.reveal v));
+  fold (nlist_hd_tl_post' p sq n input pm v input1 input2);
+  fold (nlist_hd_tl_post p sq n input pm v (input1, input2));
+  (input1, input2)
+}
+
+(* nlist_hd: get head element sub-slice *)
+
+inline_for_extraction
+fn nlist_hd
+  (#t: Type0)
+  (#k: Ghost.erased parser_kind)
+  (#p: parser k t)
+  (sq: squash (k.parser_kind_subkind == Some ParserStrong))
+  (j: LPS.jumper p)
+  (n: Ghost.erased pos)
+  (input: slice byte)
+  (#pm: perm)
+  (#v: Ghost.erased (nlist n t))
+requires
+  PPB.pts_to_parsed (parse_nlist n p) input #pm v
+returns input' : slice byte
+ensures exists* v' .
+  PPB.pts_to_parsed p input' #(pm /. 2.0R) v' **
+  trade (PPB.pts_to_parsed p input' #(pm /. 2.0R) v') (PPB.pts_to_parsed (parse_nlist n p) input #pm v) **
+  pure (
+    Cons? v /\
+    v' == List.Tot.hd v
+  )
+{
+  let (hd, tl) = nlist_hd_tl sq j n input;
+  unfold (nlist_hd_tl_post p sq n input pm v (hd, tl));
+  unfold (nlist_hd_tl_post' p sq n input pm v hd tl);
+  Trade.elim_hyp_r _ _ _;
+  hd
+}
+
+(* nlist_tl: get tail sub-slice *)
+
+inline_for_extraction
+fn nlist_tl
+  (#t: Type0)
+  (#k: Ghost.erased parser_kind)
+  (#p: parser k t)
+  (sq: squash (k.parser_kind_subkind == Some ParserStrong))
+  (j: LPS.jumper p)
+  (n: Ghost.erased pos)
+  (input: slice byte)
+  (#pm: perm)
+  (#v: Ghost.erased (nlist n t))
+requires
+  PPB.pts_to_parsed (parse_nlist n p) input #pm v
+returns input' : slice byte
+ensures exists* v' .
+  PPB.pts_to_parsed (parse_nlist (n - 1) p) input' #(pm /. 2.0R) v' **
+  trade (PPB.pts_to_parsed (parse_nlist (n - 1) p) input' #(pm /. 2.0R) v') (PPB.pts_to_parsed (parse_nlist n p) input #pm v) **
+  pure (
+    Cons? v /\
+    v' == List.Tot.tl v
+  )
+{
+  let (hd, tl) = nlist_hd_tl sq j n input;
+  unfold (nlist_hd_tl_post p sq n input pm v (hd, tl));
+  unfold (nlist_hd_tl_post' p sq n input pm v hd tl);
+  Trade.elim_hyp_l _ _ _;
+  tl
+}
